length proof and substitution lemma

Stimpfle/PumpingLemma.thy
@@ -22,14 +22,14 @@ lemma repl_length: "length (xs\<^sup>*n) = length (xs) * n"
 (* prods \<Rightarrow> Start Nt \<Rightarrow> word \<Rightarrow> path *)
 inductive path :: "('n, 't) Prods \<Rightarrow> 'n \<Rightarrow> 'n list \<Rightarrow> 't list \<Rightarrow> bool" 
    ("(2_ \<turnstile>/ (_/ \<Rightarrow>'\<langle>_'\<rangle>/ _))" [50, 0, 50] 50) where
-step:  "(A, [Tm a]) \<in> P \<Longrightarrow> P \<turnstile> A \<Rightarrow>\<langle>[A]\<rangle> [a]" |
-left:  "\<lbrakk>(A, [Nt B, Nt C]) \<in> P \<and> (P \<turnstile> B \<Rightarrow>\<langle>p\<rangle> w) \<and> (P \<turnstile> C \<Rightarrow>\<langle>q\<rangle> v)\<rbrakk> \<Longrightarrow> P \<turnstile> A \<Rightarrow>\<langle>A#p\<rangle> (w@v)" |
-right:  "\<lbrakk>(A, [Nt B, Nt C]) \<in> P \<and> (P \<turnstile> B \<Rightarrow>\<langle>p\<rangle> w) \<and> (P \<turnstile> C \<Rightarrow>\<langle>q\<rangle> v)\<rbrakk> \<Longrightarrow> P \<turnstile> A \<Rightarrow>\<langle>A#q\<rangle> (w@v)"
+terminal:  "(A, [Tm a]) \<in> P \<Longrightarrow> P \<turnstile> A \<Rightarrow>\<langle>[A]\<rangle> [a]" |
+left:  "(A, [Nt B, Nt C]) \<in> P \<Longrightarrow> (P \<turnstile> B \<Rightarrow>\<langle>p\<rangle> w) \<Longrightarrow> (P \<turnstile> C \<Rightarrow>\<langle>q\<rangle> v) \<Longrightarrow> P \<turnstile> A \<Rightarrow>\<langle>A#p\<rangle> (w@v)" |
+right:  "(A, [Nt B, Nt C]) \<in> P \<Longrightarrow> (P \<turnstile> B \<Rightarrow>\<langle>p\<rangle> w) \<Longrightarrow> (P \<turnstile> C \<Rightarrow>\<langle>q\<rangle> v) \<Longrightarrow> P \<turnstile> A \<Rightarrow>\<langle>A#q\<rangle> (w@v)"
 
 inductive cnf_derives :: "('n, 't) Prods \<Rightarrow> 'n \<Rightarrow> 't list \<Rightarrow> bool"
   ("(2_ \<turnstile>/ (_/ \<Rightarrow>cnf/ _))" [50, 0, 50] 50) where
 step:  "(A, [Tm a]) \<in> P \<Longrightarrow> P \<turnstile> A \<Rightarrow>cnf [a]"|
-trans:  "\<lbrakk>(A, [Nt B, Nt C]) \<in> P \<and> P \<turnstile> B \<Rightarrow>cnf w \<and> P \<turnstile> C \<Rightarrow>cnf v\<rbrakk> \<Longrightarrow> P \<turnstile> A \<Rightarrow>cnf (w@v)"
+trans:  "(A, [Nt B, Nt C]) \<in> P \<Longrightarrow> P \<turnstile> B \<Rightarrow>cnf w \<Longrightarrow> P \<turnstile> C \<Rightarrow>cnf v \<Longrightarrow> P \<turnstile> A \<Rightarrow>cnf (w@v)"
 
 lemma path_if_cnf_derives:
   "P \<turnstile> S \<Rightarrow>cnf w \<Longrightarrow> \<exists>p. P \<turnstile> S \<Rightarrow>\<langle>p\<rangle> w"
@@ -107,15 +107,104 @@ lemma derives_if_path:
 (* longest path *)
 inductive lpath :: "('n, 't) Prods \<Rightarrow> 'n \<Rightarrow> 'n list \<Rightarrow> 't list \<Rightarrow> bool" 
    ("(2_ \<turnstile>/ (_/ \<Rightarrow>'\<llangle>_'\<rrangle>/ _))" [50, 0, 50] 50) where
-  "(A, [Tm a]) \<in> P \<Longrightarrow> P \<turnstile> A \<Rightarrow>\<llangle>[A]\<rrangle> [a]" |
-  "\<lbrakk>(A, [Nt B, Nt C]) \<in> P \<and> (P \<turnstile> B \<Rightarrow>\<llangle>p\<rrangle> w) \<and> (P \<turnstile> C \<Rightarrow>\<llangle>q\<rrangle> v)\<rbrakk> \<Longrightarrow> 
-    P \<turnstile> A \<Rightarrow>\<llangle>A#(if length p \<ge> length q then p else q)\<rrangle> (w@v)" 
+terminal:  "(A, [Tm a]) \<in> P \<Longrightarrow> P \<turnstile> A \<Rightarrow>\<llangle>[A]\<rrangle> [a]" |
+nonTerminals:  "(A, [Nt B, Nt C]) \<in> P \<Longrightarrow> (P \<turnstile> B \<Rightarrow>\<llangle>p\<rrangle> w) \<Longrightarrow> (P \<turnstile> C \<Rightarrow>\<llangle>q\<rrangle> v) \<Longrightarrow> 
+                P \<turnstile> A \<Rightarrow>\<llangle>A#(if length p \<ge> length q then p else q)\<rrangle> (w@v)" 
 
-lemma path_lpath: "P \<turnstile> A \<Rightarrow>\<langle>p\<rangle> w \<Longrightarrow> \<exists>p'. (P \<turnstile> A \<Rightarrow>\<llangle>p'\<rrangle> w) \<and> length p' \<ge> length p"
+lemma path_lpath: "P \<turnstile> S \<Rightarrow>\<langle>p\<rangle> w \<Longrightarrow> \<exists>p'. (P \<turnstile> S \<Rightarrow>\<llangle>p'\<rrangle> w) \<and> length p' \<ge> length p"
   by (induction rule: path.induct) (auto intro: lpath.intros)
 
-lemma lpath_path: "(P \<turnstile> A \<Rightarrow>\<llangle>p\<rrangle> w) \<Longrightarrow> P \<turnstile> A \<Rightarrow>\<langle>p\<rangle> w"
+lemma lpath_path: "(P \<turnstile> S \<Rightarrow>\<llangle>p\<rrangle> w) \<Longrightarrow> P \<turnstile> S \<Rightarrow>\<langle>p\<rangle> w"
   by (induction rule: lpath.induct) (auto intro: path.intros)
+
+(*Property of the derivation tree: 
+Since the tree is a binary tree, word lengths are always \<le> 2^longest path*)
+lemma lpath_length: "(P \<turnstile> S \<Rightarrow>\<llangle>p\<rrangle> w) \<Longrightarrow> length w \<le> 2^length p"
+proof (induction rule: lpath.induct)
+  case (terminal A a P)
+  then show ?case by simp
+next
+  case (nonTerminals A B C P p w q v)
+  then show ?case 
+  proof (cases "length p \<ge> length q")
+    case True
+    hence "length v \<le> 2^length p"
+      using nonTerminals(5) order_subst1[of \<open>length v\<close> \<open>\<lambda>x. 2^x\<close> \<open>length q\<close> \<open>length p\<close>] by simp
+    hence "length w +length v \<le> 2*2^length p"
+      by (simp add: nonTerminals.IH(1) add_le_mono mult_2)
+    then show ?thesis
+      by (simp add: True)
+  next
+    case False
+    hence "length w \<le> 2^length q"
+      using nonTerminals(4) order_subst1[of \<open>length w\<close> \<open>\<lambda>x. 2^x\<close> \<open>length p\<close> \<open>length q\<close>] by simp 
+    hence "length w +length v \<le> 2*2^length q"
+      by (simp add: nonTerminals.IH(2) add_le_mono mult_2)
+    then show ?thesis
+      by (simp add: False)
+  qed
+qed
+
+(*auxiliary lemma: if A\<rightarrow>*wv using a#p and length a#p \<ge> 1 then the derivation can be decomposed:
+there exist B C where B\<rightarrow>*w and C\<rightarrow>*v and A\<rightarrow>BC and one of both derivation uses the path p. *)
+lemma step_decomp:
+  assumes "P \<turnstile> A \<Rightarrow>\<langle>[A]@p\<rangle> w" " length p \<ge> 1" 
+  shows "\<exists>B C p' a b. (A, [Nt B, Nt C]) \<in> P \<and> w =a@b \<and>
+        (((P \<turnstile> B \<Rightarrow>\<langle>p\<rangle> a) \<and> (P \<turnstile> C \<Rightarrow>\<langle>p'\<rangle> b)) \<or> ((P \<turnstile> B \<Rightarrow>\<langle>p'\<rangle> a) \<and> (P \<turnstile> C \<Rightarrow>\<langle>p\<rangle> b)))"
+  using assms by (cases) fastforce+
+
+lemma steplp_decomp:
+  assumes "P \<turnstile> A \<Rightarrow>\<llangle>[A]@p\<rrangle> w" " length p \<ge> 1" 
+  shows "\<exists>B C p' a b. (A, [Nt B, Nt C]) \<in> P \<and> w =a@b \<and>
+      (((P \<turnstile> B \<Rightarrow>\<llangle>p\<rrangle> a) \<and> (P \<turnstile> C \<Rightarrow>\<llangle>p'\<rrangle> b) \<and> length p \<ge> length p') \<or>
+      ((P \<turnstile> B \<Rightarrow>\<llangle>p'\<rrangle> a) \<and> (P \<turnstile> C \<Rightarrow>\<llangle>p\<rrangle> b) \<and> length p \<ge> length p'))"
+  using assms by (cases) fastforce+
+
+(*first Nonterminal in the path is root node*)
+lemma path_first_step: "P \<turnstile> A \<Rightarrow>\<langle>p\<rangle> w \<Longrightarrow> \<exists>q. p = [A]@q "
+  by (induction rule: path.induct) simp_all
+
+lemma no_empty: "P \<turnstile> A \<Rightarrow>\<langle>p\<rangle> w \<Longrightarrow> length w > 0"
+  by (induction rule: path.induct) simp_all
+
+(*if A\<rightarrow>*z using p1Xp2 then z can be decomposed into v w x where X\<rightarrow>*w and if X\<rightarrow>*w' then A\<rightarrow>*vw'x.
+v and x are universal, i.e. they are independent from arbitrary w'.
+If the front part p1 is not empty then v or x is not empty.*)
+lemma substitution: 
+  assumes "P \<turnstile> A \<Rightarrow>\<langle>p1@[X]@p2\<rangle> z"
+  shows "\<exists>v w x. ((P \<turnstile> X \<Rightarrow>\<langle>[X]@p2\<rangle> w) \<and> z = v@w@x \<and>
+        (\<forall>subst p'. ((P \<turnstile> X \<Rightarrow>\<langle>[X]@p'\<rangle> subst) \<longrightarrow> P \<turnstile> A \<Rightarrow>\<langle>p1@[X]@p'\<rangle> v@subst@x)) \<and>
+        (length p1 > 0 \<longrightarrow> length (v@x) > 0))"
+using assms proof (induction p1 arbitrary: P A z X p2)
+  case Nil
+  hence "\<forall>subst p'. ((P \<turnstile> X \<Rightarrow>\<langle>[X]@p2\<rangle> z) \<and> z = []@z@[] \<and>
+        ((P \<turnstile> X \<Rightarrow>\<langle>[X]@p'\<rangle> subst) \<longrightarrow> P \<turnstile> A \<Rightarrow>\<langle>[]@[X]@p'\<rangle> ([]@subst@[])) \<and>
+        (length [] > 0 \<longrightarrow> length ([]@[]) > 0))"
+    using path_first_step[of P A] by auto
+  then show ?case 
+    by blast
+next
+  case (Cons A p1 P Y)
+  hence 0: "A = Y"
+    using path_first_step[of P Y] by fastforce 
+  have "length (p1@[X]@p2) \<ge> 1"
+    by simp
+  hence "\<exists>B C a b q. (A, [Nt B, Nt C]) \<in> P \<and> a@b = z \<and> 
+        (((P \<turnstile> B \<Rightarrow>\<langle>q\<rangle> a) \<and> P \<turnstile> C \<Rightarrow>\<langle>p1@[X]@p2\<rangle> b) \<or> ((P \<turnstile> B \<Rightarrow>\<langle>p1@[X]@p2\<rangle> a) \<and> P \<turnstile> C \<Rightarrow>\<langle>q\<rangle> b))"
+    using Cons.prems path_first_step step_decomp by fastforce
+  from this obtain B C a b q where ttree: "(A, [Nt B, Nt C]) \<in> P \<and> a@b = z \<and> 
+        (((P \<turnstile> B \<Rightarrow>\<langle>q\<rangle> a) \<and> P \<turnstile> C \<Rightarrow>\<langle>p1@[X]@p2\<rangle> b) \<or> ((P \<turnstile> B \<Rightarrow>\<langle>p1@[X]@p2\<rangle> a) \<and> P \<turnstile> C \<Rightarrow>\<langle>q\<rangle> b))"
+    by blast
+  then show ?case
+  proof (cases "((P \<turnstile> B \<Rightarrow>\<langle>q\<rangle> a) \<and> P \<turnstile> C \<Rightarrow>\<langle>p1@[X]@p2\<rangle> b)")
+    case True
+    then show ?thesis sorry
+  next
+    case False
+    then show ?thesis sorry
+  qed
+qed
+
 
 (* towards pumping lemma *)
 lemma inner_pumping: 
